fix the definition but weird syntax error

prover/theories/Named.v
@@ -207,65 +207,76 @@ Defined.
     := sg_next sg (named_free_svars ϕ)
   .
 
-  Definition named_fresh_evar' avoid ϕ := evar_fresh (elements (named_evars ϕ ∪ avoid)).
-  Definition named_fresh_svar' avoid ϕ := svar_fresh (elements (named_svars ϕ ∪ avoid)).
-  (*Definition named_fresh_evar ϕ := named_fresh_evar' ∅ ϕ.
-  Definition named_fresh_svar ϕ := named_fresh_svar' ∅ ϕ.*)
-
   (* substitute variable x for psi in phi: phi[psi/x] *)
   Fixpoint named_evar_subst'
-    (eg : EVarGen) (phi psi : NamedPattern) (x : evar) :=
+    (eg : EVarGen) (phi psi : NamedPattern) (x : evar) : NamedPattern :=
     match phi with
     | npatt_evar x' => if decide (x = x') is left _ then psi else npatt_evar x'
     | npatt_svar X => npatt_svar X
     | npatt_sym sigma => npatt_sym sigma
-    | npatt_app phi1 phi2 => npatt_app (named_evar_subst' avoid phi1 psi x)
-                                       (named_evar_subst' avoid phi2 psi x)
+    | npatt_app phi1 phi2 => npatt_app (named_evar_subst' eg phi1 psi x)
+                                       (named_evar_subst' eg phi2 psi x)
     | npatt_bott => npatt_bott
-    | npatt_imp phi1 phi2 => npatt_imp (named_evar_subst' avoid phi1 psi x)
-                                       (named_evar_subst' avoid phi2 psi x)
-    | npatt_exists x' phi' => if decide (x = x') is left _
-                              then let fx := named_fresh_evar' avoid phi' in
-                                   npatt_exists fx (named_evar_subst' (avoid ∪ {[fx]}) phi' (npatt_evar fx) x)
-                              else npatt_exists x' (named_evar_subst' avoid phi' psi x)
-    | npatt_mu X phi' => npatt_mu X (named_evar_subst' avoid phi' psi x)
+    | npatt_imp phi1 phi2 => npatt_imp (named_evar_subst' eg phi1 psi x)
+                                       (named_evar_subst' eg phi2 psi x)
+    | npatt_exists x' phi'
+      => (if (decide (x = x')) is left _
+         then (npatt_exists x' phi') (* no-op *)
+         else (
+          if (decide (x' ∈ named_free_evars ψ)) is left _
+          then (
+            let avoid := union (named_free_evars ψ) (named_free_evars ϕ') in
+            let fresh_x := eg_get eg avoid in
+            (*let new_eg := eg_next avoid in*)
+            let renamed_phi' := (named_evar_subst' eg phi' (npatt_evar fresh_x) x) in
+            in (
+              npatt_bott
+              npatt_exists fresh_x (named_evar_subst' eg renamed_phi' ψ x)
+            )
+          )
+          else
+            npatt_exists x' (named_evar_subst' eg phi' ψ x)
+         ))
+    | npatt_mu X phi'
+      => npatt_mu X (named_evar_subst' eg phi' psi x)
     end.
 
   (* substitute variable X for psi in phi: phi[psi/X] *)
   Fixpoint named_svar_subst'
-    (avoid : gset svar)
+    (sg : SVarGen)
     (phi psi : NamedPattern) (X : svar) :=
     match phi with
     | npatt_evar x => npatt_evar x
     | npatt_svar X' => if decide (X = X') is left _ then psi else npatt_svar X'
     | npatt_sym sigma => npatt_sym sigma
-    | npatt_app phi1 phi2 => npatt_app (named_svar_subst' avoid phi1 psi X)
-                                       (named_svar_subst' avoid phi2 psi X)
+    | npatt_app phi1 phi2 => npatt_app (named_svar_subst' sg phi1 psi X)
+                                       (named_svar_subst' sg phi2 psi X)
     | npatt_bott => npatt_bott
-    | npatt_imp phi1 phi2 => npatt_imp (named_svar_subst' avoid phi1 psi X)
-                                       (named_svar_subst' avoid phi2 psi X)
-    | npatt_exists x phi' => npatt_exists x (named_svar_subst' avoid phi' psi X)
+    | npatt_imp phi1 phi2 => npatt_imp (named_svar_subst' sg phi1 psi X)
+                                       (named_svar_subst' sg phi2 psi X)
+    | npatt_exists x phi' => npatt_exists x (named_svar_subst' sg phi' psi X)
     | npatt_mu X' phi' => if decide (X = X') is left _
-                          then let fX := named_fresh_svar' avoid phi' in
-                               npatt_mu fX (named_svar_subst' (avoid ∪ {[fX]}) phi' (npatt_svar fX) X)
-                          else npatt_mu X' (named_svar_subst' avoid phi' psi X)
+                          then let fX := sg_getf sg phi' in
+                               npatt_mu fX (named_svar_subst' (sg_nextf sg phi') phi' (npatt_svar fX) X)
+                          else npatt_mu X' (named_svar_subst' sg phi' psi X)
     end.
 
   Definition named_evar_subst
     (phi psi : NamedPattern) (x : evar) : NamedPattern
-    := named_evar_subst' ∅ phi psi x
+    := named_evar_subst' (default_EVarGen ∅) phi psi x
   .
+
   Definition named_svar_subst
     (phi psi : NamedPattern) (X : svar) : NamedPattern
-    := named_svar_subst' ∅ phi psi X
+    := named_svar_subst' (default_SVarGen ∅) phi psi X
   .
 
   Lemma nsize_named_evar_subst_evar'
-    avoid (ϕ : NamedPattern) (x y : evar):
-    nsize' (named_evar_subst' avoid ϕ (npatt_evar y) x) = nsize' ϕ.
+    eg (ϕ : NamedPattern) (x y : evar):
+    nsize' (named_evar_subst' eg ϕ (npatt_evar y) x) = nsize' ϕ.
   Proof.
-    move: x y avoid.
-    induction ϕ; intros x' y avoid; cbn; try reflexivity.
+    move: x y eg.
+    induction ϕ; intros x' y eg; cbn; try reflexivity.
     {
       destruct (decide (x' = x)); reflexivity.
     }
@@ -290,11 +301,11 @@ Defined.
   Qed.
 
   Lemma nsize_named_evar_subst_svar'
-    avoid (ϕ : NamedPattern) (X Y : svar):
-    nsize' (named_svar_subst' avoid ϕ (npatt_svar Y) X) = nsize' ϕ.
+    sg (ϕ : NamedPattern) (X Y : svar):
+    nsize' (named_svar_subst' sg ϕ (npatt_svar Y) X) = nsize' ϕ.
   Proof.
-    move: X Y avoid.
-    induction ϕ; intros X' Y avoid; cbn; try reflexivity.
+    move: X Y sg.
+    induction ϕ; intros X' Y sg; cbn; try reflexivity.
     {
       destruct (decide (X' = X)); reflexivity.
     }
@@ -318,13 +329,13 @@ Defined.
     }
   Qed.
 
-  Lemma named_evar_subst_noop avoid (ϕ : NamedPattern) (x : evar) :
+  Lemma named_evar_subst_noop sg (ϕ : NamedPattern) (x : evar) :
     x ∉ named_evars ϕ ->
-    named_evar_subst' avoid ϕ (npatt_evar x) x = ϕ
+    named_evar_subst' sg ϕ (npatt_evar x) x = ϕ
   .
   Proof.
-    move: x avoid.
-    induction ϕ; intros x' avoid Hx'; cbn; try reflexivity.
+    move: x sg.
+    induction ϕ; intros x' sg Hx'; cbn; try reflexivity.
     {
       destruct (decide (x' = x)).
       { subst. reflexivity. }
@@ -332,14 +343,14 @@ Defined.
     }
     {
       cbn in Hx'.
-      specialize (IHϕ1 x' avoid ltac:(set_solver)).
-      specialize (IHϕ2 x' avoid ltac:(set_solver)).
+      specialize (IHϕ1 x' sg ltac:(set_solver)).
+      specialize (IHϕ2 x' sg ltac:(set_solver)).
       congruence.
     }
     {
       cbn in Hx'.
-      specialize (IHϕ1 x' avoid ltac:(set_solver)).
-      specialize (IHϕ2 x' avoid ltac:(set_solver)).
+      specialize (IHϕ1 x' sg ltac:(set_solver)).
+      specialize (IHϕ2 x' sg ltac:(set_solver)).
       congruence.
     }
     {
@@ -361,20 +372,20 @@ Defined.
   Qed.
 
   Lemma named_evar_subst_chain
-    avoid1 avoid2 (ϕ ψ: NamedPattern) (x y : evar) :
+    eg1 eg2 (ϕ ψ: NamedPattern) (x y : evar) :
     y ∉ named_evars ϕ ->
-    named_evar_subst' avoid2 (named_evar_subst' avoid1 ϕ (npatt_evar y) x) ψ y
-    = named_evar_subst' avoid2 ϕ ψ x
+    named_evar_subst' eg2 (named_evar_subst' eg1 ϕ (npatt_evar y) x) ψ y
+    = named_evar_subst' eg2 ϕ ψ x
   .
   Proof.
-    move: avoid1 avoid2 x y ψ.
+    move: eg1 eg2 x y ψ.
     remember (nsize' ϕ) as sz.
     assert (Hsz: nsize' ϕ <= sz) by lia.
     clear Heqsz.
     move: ϕ Hsz.
     induction sz; cbn; intros ϕ Hsz.
     { destruct ϕ; cbn in Hsz; lia. }
-    destruct ϕ; intros avoid1 avoid2 x' y ψ Hfry; cbn; try reflexivity.
+    destruct ϕ; intros eg1 eg2 x' y ψ Hfry; cbn; try reflexivity.
     {
       destruct (decide (x' = x)).
       { subst. cbn. rewrite decide_eq_same. reflexivity. }
@@ -409,12 +420,16 @@ Defined.
       destruct (decide (x' = x)).
       {
         subst. cbn.
-        destruct (decide (y = named_fresh_evar' avoid1 ϕ)).
+        destruct (decide (y = eg_getf eg1 ϕ)).
         {
           subst.
           rewrite IHsz.
           { lia. }
           { set_solver. }
+          f_equal.
+          {
+            unfold eg_getf.
+          }
           cut (named_fresh_evar' avoid2 ϕ = named_fresh_evar' avoid2 (named_evar_subst' (avoid1 ∪ {[named_fresh_evar' avoid1 ϕ]}) ϕ (npatt_evar (named_fresh_evar' avoid1 ϕ)) x)).
           { intros H.
             congruence.
